nsl_dh.v
@@ -26,13 +26,13 @@ Ltac protocol_failure :=
   by intros; wp_pures; iApply ("Hpost" $! None).
 
 Definition nsl_dh_init : val := λ: "g" "skA" "pkA" "pkB",
-  let: "a" := mknonce #() in
+  let: "a" := mkdh #() in
   let: "ga" := texp (tgroup "g") "a" in
   bind: "gb" := nsl_init (N.@"nsl") "skA" "pkA" "pkB" "ga" in
   SOME (texp "gb" "a").
 
 Definition nsl_dh_resp : val := λ: "g" "skB" "pkB",
-  let: "b" := mknonce #() in
+  let: "b" := mkdh #() in
   let: "gb" := texp (tgroup "g") "b" in
   bind: "res" := nsl_resp (N.@"nsl") "skB" "pkB" "gb" in
   let: "pkA" := Fst "res" in
@@ -53,30 +53,30 @@ Definition nsl_dh_inv g rl kA kB ga gb : iProp :=
   end%I.
 
 Definition nsl_dh_fail (k : term) a : iProp :=
-  ∃ k', meta a (N.@"peer") k' ∧ corruption k k'.
+  ∃ k', crypto_meta a (N.@"peer") k' ∧ corruption k k'.
 
 Lemma pterm_nsl_dh1 g a k k' :
   dh_gen g -∗
-  dh_nonce (nsl_dh_fail k) a -∗
-  meta a (N.@"peer") k' -∗
-  pterm (TExp g [TNonce a])  ↔ ▷ corruption k k'.
+  dh_seed (nsl_dh_fail k) a -∗
+  crypto_meta a (N.@"peer") k' -∗
+  pterm (TExp g [a])  ↔ ▷ corruption k k'.
 Proof.
 iIntros "#gP #a_pred #meta"; iSplit.
 - iIntros "#p_e".
-  iDestruct (dh_nonce_elim1 with "a_pred p_e") as (k'') "[meta' corr]".
+  iDestruct (dh_seed_elim1 with "a_pred p_e") as (k'') "[meta' corr]".
   iModIntro.
-  by iPoseProof (meta_agree with "meta meta'") as "<-".
+  by iPoseProof (crypto_meta_agree with "meta meta'") as "<-".
 - iIntros "#corr".
   iApply dh_pterm_TExp; eauto.
   by iExists k'; iModIntro; iModIntro; iSplit; eauto.
 Qed.
 
 Lemma pterm_nsl_dh2 g a k t :
-  dh_nonce (nsl_dh_fail k) a -∗
-  pterm (TExp g [TNonce a; t]) -∗ ◇ pterm t.
+  dh_seed (nsl_dh_fail k) a -∗
+  pterm (TExp g [a; t]) -∗ ◇ pterm t.
 Proof.
 iIntros "#a_pred #p_e".
-by iPoseProof (dh_nonce_elim2 with "a_pred p_e") as ">[??]".
+by iPoseProof (dh_seed_elim2 with "a_pred p_e") as ">[??]".
 Qed.
 
 Lemma wp_nsl_dh_init g kA kB E Ψ :
@@ -96,11 +96,11 @@ Lemma wp_nsl_dh_init g kA kB E Ψ :
 Proof.
 iIntros (?? g0) "#ctx #p_e_kA #p_e_kB Hpost".
 rewrite /nsl_dh_init; wp_pures; wp_bind (mknonce _).
-iApply (wp_mknonce _ (dh_pred (nsl_dh_fail kA))).
+iApply (wp_mkdh (nsl_dh_fail kA)).
 iIntros (a) "#s_a #a_pred token".
-rewrite (meta_token_difference _ (↑N.@"peer")); last solve_ndisj.
+rewrite (crypto_meta_token_difference _ (↑N.@"peer")); last solve_ndisj.
 iDestruct "token" as "[dh token]".
-iMod (meta_set _ _ kB with "dh") as "#dh"; eauto.
+iMod (crypto_meta_set _ _ _ kB with "dh") as "#dh"; eauto.
 wp_pures; wp_bind (tgroup _); iApply wp_tgroup.
 wp_pures; wp_bind (texp _ _); iApply wp_texp.
 rewrite Spec.texpA; wp_pures; wp_bind (nsl_init _ _ _ _ _).
@@ -111,31 +111,28 @@ iApply (wp_nsl_init with "ctx p_e_kA p_e_kB [] [] [] [token]") => //.
   by rewrite /=; iSplit.
 - by iModIntro; iApply pterm_nsl_dh1; eauto; iApply nonces_of_term_dh_gen.
 - iIntros (nB); rewrite /=.
-  iExists (TNonce a); iSplit => //.
+  iExists a; iSplit => //.
   iModIntro; iIntros (b) "p_b".
   by iApply pterm_nsl_dh2.
-- rewrite /crypto_meta_token nonces_of_term_TExp /=.
-  rewrite g0 nonces_of_term_eq right_id_L left_id_L /=.
-  iSplit; first by iPureIntro; set_solver.
-  rewrite big_sepS_singleton.
-  rewrite (meta_token_difference _ (↑N.@"nsl")).
-    by iDestruct "token" as "[??]".
-  by solve_ndisj.
+- rewrite (crypto_meta_token_difference _ (↑N.@"nsl")); last solve_ndisj.
+  iDestruct "token" as "[token _]".
+  rewrite /crypto_meta_token nonces_of_term_TExp /=.
+  by rewrite g0 nonces_of_term_eq right_id_L left_id_L /=.
 iIntros (onB) "pub"; case: onB=> [nB|]; last by protocol_failure.
 iDestruct "pub" as "# [s_nB [fail | succ]]".
   wp_pures; wp_bind (texp _ _); iApply wp_texp; wp_pures.
-  iApply ("Hpost" $! (Some (Spec.texp nB (TNonce a)))).
+  iApply ("Hpost" $! (Some (Spec.texp nB a))).
   iSplit; first by iApply sterm_texp => //.
   by eauto.
 iDestruct "succ" as (b) "[-> #succ]".
 wp_pures; wp_bind (texp _ _); iApply wp_texp; wp_pures.
-iApply ("Hpost" $! (Some (Spec.texp (TExp g [b]) (TNonce a)))).
+iApply ("Hpost" $! (Some (Spec.texp (TExp g [b]) a))).
 iSplit; first by iApply sterm_texp => //.
 iRight; iModIntro.
 rewrite Spec.texpA.
 iIntros "#contra".
 iDestruct ("succ" with "contra") as "{succ} >succ".
-by iApply dh_nonce_elim0.
+by iApply dh_seed_elim0.
 Qed.
 
 Lemma wp_dh_responder g kB E Ψ :
@@ -156,48 +153,45 @@ Lemma wp_dh_responder g kB E Ψ :
   WP nsl_dh_resp g (TKey Dec kB) (TKey Enc kB) @ E {{ Ψ }}.
 Proof.
 iIntros (?? g0) "#ctx #p_e_kB Hpost".
-rewrite /nsl_dh_resp; wp_pures; wp_bind (mknonce _).
-iApply (wp_mknonce _ (dh_pred (nsl_dh_fail kB))).
+rewrite /nsl_dh_resp; wp_pures; wp_bind (mkdh _).
+iApply (wp_mkdh (nsl_dh_fail kB)).
 iIntros (b) "#s_b #b_pred token".
-rewrite (meta_token_difference _ (↑N.@"peer")); last solve_ndisj.
+rewrite (crypto_meta_token_difference _ (↑N.@"peer")); last solve_ndisj.
 iDestruct "token" as "[dh token]".
 wp_pures; wp_bind (tgroup _); iApply wp_tgroup.
 wp_pures; wp_bind (texp _ _); iApply wp_texp.
 rewrite Spec.texpA; wp_pures; wp_bind (nsl_resp _ _ _ _).
 iApply (wp_nsl_resp with "ctx p_e_kB [token] [] [dh]") => //.
 - solve_ndisj.
-- rewrite /crypto_meta_token nonces_of_term_TExp /=.
-  rewrite g0 nonces_of_term_eq right_id_L left_id_L /=.
-  iSplit; first by iPureIntro; set_solver.
-  rewrite big_sepS_singleton.
-  rewrite (meta_token_difference _ (↑N.@"nsl")).
-    by iDestruct "token" as "[??]".
-  by solve_ndisj.
+- rewrite (crypto_meta_token_difference _ (↑N.@"nsl")); last solve_ndisj.
+  iDestruct "token" as "[token _]".
+  rewrite /crypto_meta_token nonces_of_term_TExp /=.
+  by rewrite g0 nonces_of_term_eq right_id_L left_id_L /=.
 - rewrite sterm_TExp /=; iSplit; eauto.
   by iApply dh_gen_sterm; iApply nonces_of_term_dh_gen.
 - iIntros (kA nA).
-  iMod (meta_set _ b kA with "dh") as "#meta"; eauto.
+  iMod (crypto_meta_set _ _ _ kA with "dh") as "#meta"; eauto.
   iModIntro; iSplit.
   + iModIntro; rewrite [corruption _ _]comm.
     by iApply pterm_nsl_dh1 => //; iApply nonces_of_term_dh_gen.
-  + iExists (TNonce b); iSplit => //.
+  + iExists b; iSplit => //.
     iIntros "!> %".
-    rewrite -[ [a; TNonce b]]/(seq.cat [a] [TNonce b]) TExpC /=.
+    rewrite -[ [a; b]]/(seq.cat [a] [b]) TExpC /=.
     by iIntros "#?"; iApply pterm_nsl_dh2.
 iIntros ([[pkA nA]|]) "resp"; last by protocol_failure.
 iDestruct "resp" as (kA) "# (-> & p_e_kA & s_nA & p_nA & inv)".
 wp_pures; wp_bind (texp _ _); iApply wp_texp; wp_pures.
-iApply ("Hpost" $! (Some (TKey Enc kA, Spec.texp nA (TNonce b)))).
+iApply ("Hpost" $! (Some (TKey Enc kA, Spec.texp nA b))).
 iExists _; do 3!iSplit => //; eauto.
   by iApply sterm_texp.
 iDestruct "inv" as "[inv|inv]"; eauto.
 iDestruct "inv" as (t) "[-> #inv]".
 rewrite Spec.texpA.
-rewrite -[ [TNonce b; t]]/(seq.cat [TNonce b] [t]) TExpC /=.
+rewrite -[ [b; t]]/(seq.cat [b] [t]) TExpC /=.
 iRight; iIntros "!> #contra".
 iSpecialize ("inv" with "contra").
 iDestruct "inv" as ">inv".
-by iApply dh_nonce_elim0.
+by iApply dh_seed_elim0.
 Qed.
 
 End NSLDH.
